

$$\begin{aligned}
m_1 \ddot{z}_1 + c_1(\dot{z}_1 - \dot{z}_2) + k_1(z_1 - z_2) &= 0, \\
m_2 \ddot{z}_2 + c_1(\dot{z}_2 - \dot{z}_1) + c_2(\dot{z}_2 - \dot{h}) + k_1(z_2 - z_1) + k_2(z_2 - h) &= 0.
\end{aligned}$$

$$\begin{aligned}
\dot{z}_1 &= z_3, \\
\dot{z}_2 &= z_4, \\
\dot{z}_3 &= \frac{1}{m_1} \left( -k_1 z_1 + k_1 z_2 - c_1 z_3 + c_1 z_4 \right), \\
\dot{z}_4 &= \frac{1}{m_2} \left( k_1 z_1 - (k_1 + k_2) z_2 + c_1 z_3 - (c_1 + c_2) z_4 + k_2 h + c_2 \dot{h} \right).
\end{aligned}$$

$$\frac{d}{dt} \begin{pmatrix} z_1 \\ z_2 \\ z_3 \\ z_4 \end{pmatrix} = \begin{pmatrix} 0 & 0 & 1 & 0 \\ 0 & 0 & 0 & 1 \\ -k_1/m_1 & k_1/m_1 & -c_1/m_1 & c_1/m_1 \\ k_1/m_2 & -(k_1 + k_2)/m_2 & c_1/m_2 & -(c_1 + c_2)/m_2 \end{pmatrix} \begin{pmatrix} z_1 \\ z_2 \\ z_3 \\ z_4 \end{pmatrix} + \begin{pmatrix} 0 \\ 0 \\ 0 \\ (k_2 h + c_2 \dot{h})/m_2 \end{pmatrix}.$$

$$h(t) = \begin{cases} \frac{H}{2} \left( 1 - \cos \left( \frac{2\pi u t}{L} \right) \right), & t \leq \frac{L}{u}, \\ 0, & t > \frac{L}{u}. \end{cases}$$

$$\dot{h}(t) = \begin{cases} \frac{H}{2} \frac{2\pi u}{L} \sin \left( \frac{2\pi u t}{L} \right), & t \leq \frac{L}{u}, \\ 0, & t > \frac{L}{u}. \end{cases}$$

$$\mathbf{g}(t) = \begin{cases} \begin{pmatrix} 0 \\ 0 \\ 0 \\ \frac{k_2}{m_2} \frac{H}{2} \left( 1 - \cos \left( \frac{2\pi u t}{L} \right) \right) + \frac{c_2}{m_2} \frac{H}{2} \frac{2\pi u}{L} \sin \left( \frac{2\pi u t}{L} \right) \end{pmatrix}, & t \leq \frac{L}{u}, \\ \begin{pmatrix} 0 \\ 0 \\ 0 \\ 0 \end{pmatrix}, & t > \frac{L}{u}. \end{cases}$$